<?xml version="1.0" encoding="utf-8"?>
<rdf:RDF xmlns:dcterms="http://purl.org/dc/terms/" xmlns:foaf="http://xmlns.com/foaf/0.1/"
         xmlns:prov="http://www.w3.org/ns/prov#"
         xmlns:skos="http://www.w3.org/2004/02/skos/core#"
         xmlns:xkos="http://purl.org/linked-data/xkos#"
         xmlns:pso="http://www.patexpert.org/ontologies/pso.owl#"
         xmlns:rdf="http://www.w3.org/1999/02/22-rdf-syntax-ns#"
         xmlns:pulo="http://www.patexpert.org/ontologies/pulo.owl#"
         xmlns:rdfs="http://www.w3.org/2000/01/rdf-schema#"
         xmlns:sumo="http://www.owl-ontologies.com/sumo.owl#"
         xmlns:owl="http://www.w3.org/2002/07/owl#"
         xmlns:pmo="http://www.patexpert.org/ontologies/pmo.owl#"
         xmlns:xsd="http://www.w3.org/2001/XMLSchema#"
         xmlns:property="http://example.org/property/"
         xmlns:schema="http://schema.org/">
   <rdf:Description rdf:about="http://csarven.ca/#i">
      <rdf:type rdf:resource="http://www.w3.org/ns/prov#Agent"/>
   </rdf:Description>
   <rdf:Description xmlns:xs="http://www.w3.org/2001/XMLSchema"
                    rdf:about="http://example.org/provenance/activity/20130221095651">
      <rdf:type rdf:resource="http://www.w3.org/ns/prov#Activity"/>
      <prov:startedAtTime rdf:datatype="http://www.w3.org/2001/XMLSchema#dateTime">2013-02-21T09:56:51Z</prov:startedAtTime>
      <prov:wasAssociatedWith rdf:resource="http://csarven.ca/#i"/>
      <prov:used rdf:resource="http://example.org/data/US-H1-H.xml"/>
      <prov:used rdf:resource="https://github.com/fusepool/patents-reengineering/src/main/resources/scripts/marec.xsl"/>
      <prov:generated>
         <rdf:Description rdf:about="http://example.org/patent/US-H1-H">
            <prov:wasDerivedFrom rdf:resource="http://example.org/data/US-H1-H.xml"/>
            <prov:wasGeneratedBy rdf:resource="http://example.org/provenance/activity/20130221095651"/>
         </rdf:Description>
      </prov:generated>
   </rdf:Description>
   <rdf:Description rdf:about="http://example.org/patent/US-H1-H">
      <rdf:type rdf:resource="http://www.owl-ontologies.com/sumo.owl#Patent"/>
      <property:status>new</property:status>
      <pmo:patentFamily>
         <rdf:Description rdf:about="http://example.org/family/24343680">
            <rdf:type rdf:resource="http://www.patexpert.org/ontologies/pmo.owl#PatentFamily"/>
            <rdf:type rdf:resource="http://www.w3.org/2004/02/skos/core#Collection"/>
            <skos:notation>24343680</skos:notation>
         </rdf:Description>
      </pmo:patentFamily>
   </rdf:Description>
   <rdf:Description rdf:about="http://example.org/patent/US-H1-H">
      <dcterms:references>
         <rdf:Description rdf:about="http://example.org/patent/US-H1-H/publication">
            <rdf:type rdf:resource="http://www.patexpert.org/ontologies/pmo.owl#IntellectualPropertyDocument"/>
            <property:status>new</property:status>
            <dcterms:hasPart>
               <rdf:Description rdf:about="http://example.org/patent/US-H1-H/publication/19851203">
                  <rdf:type rdf:resource="http://www.patexpert.org/ontologies/pmo.owl#PatentPublication"/>
                  <dcterms:isPartOf rdf:resource="http://example.org/patent/US-H1-H/publication"/>
                  <property:status>new</property:status>
                  <pulo:fileFormat>original</pulo:fileFormat>
                  <property:filing-office rdf:resource="http://example.org/code/filing-office/US"/>
                  <pmo:publicationNumber>H1</pmo:publicationNumber>
                  <pmo:dateOfPublication rdf:datatype="http://www.w3.org/2001/XMLSchema#date">1985-12-03</pmo:dateOfPublication>
               </rdf:Description>
            </dcterms:hasPart>
         </rdf:Description>
      </dcterms:references>
   </rdf:Description>
   <rdf:Description rdf:about="http://example.org/patent/US-H1-H">
      <dcterms:references>
         <rdf:Description rdf:about="http://example.org/patent/US-58595184-A/application">
            <rdf:type rdf:resource="http://www.patexpert.org/ontologies/pmo.owl#IntellectualPropertyDocument"/>
            <property:status>new</property:status>
            <property:appl-type>7</property:appl-type>
            <property:us-series-code>6 </property:us-series-code>
            <property:us-art-unit>221</property:us-art-unit>
            <property:is-representative>NO</property:is-representative>
            <dcterms:hasPart>
               <rdf:Description rdf:about="http://example.org/patent/US-58595184-A/application/19840305">
                  <rdf:type rdf:resource="http://www.patexpert.org/ontologies/pmo.owl#PatentPublication"/>
                  <dcterms:isPartOf rdf:resource="http://example.org/patent/US-58595184-A/application"/>
                  <property:status>new</property:status>
                  <pulo:fileFormat>epo</pulo:fileFormat>
                  <property:filing-office rdf:resource="http://example.org/code/filing-office/US"/>
                  <pmo:applicationNumber>58595184</pmo:applicationNumber>
                  <pmo:dateOfPublication rdf:datatype="http://www.w3.org/2001/XMLSchema#date">1984-03-05</pmo:dateOfPublication>
               </rdf:Description>
            </dcterms:hasPart>
         </rdf:Description>
      </dcterms:references>
   </rdf:Description>
   <rdf:Description rdf:about="http://example.org/patent/US-H1-H">
      <property:priority-claim>
         <rdf:Description rdf:about="http://example.org/patent/US-58595184-A/publication/1">
            <rdf:type rdf:resource="http://www.patexpert.org/ontologies/pmo.owl#PatentPublication"/>
         </rdf:Description>
      </property:priority-claim>
   </rdf:Description>
   <rdf:Description rdf:about="http://example.org/patent/US-H1-H">
      <pmo:classifiedAs>
         <rdf:Description rdf:about="http://example.org/concept/ecla/H01R4/24B3D1">
            <rdf:type rdf:resource="http://www.w3.org/2004/02/skos/core#Concept"/>
            <pmo:classifiedPatent rdf:resource="http://example.org/patent/US-H1-H"/>
            <pmo:classifiedPatent rdf:resource="http://example.org/concept/H01R4/24B3D1"/>
            <pmo:classificationCode>H01R4/24B3D1</pmo:classificationCode>
            <skos:notation>H01R4/24B3D1</skos:notation>
         </rdf:Description>
      </pmo:classifiedAs>
   </rdf:Description>
   <rdf:Description rdf:about="http://example.org/patent/US-H1-H">
      <dcterms:title xml:lang="en">Split barrel insulation displacing connector</dcterms:title>
   </rdf:Description>
   <rdf:Description rdf:about="http://example.org/patent/US-H1-H">
      <pmo:inventor>
         <rdf:Description rdf:about="urn:uuid:43f5d708-bf15-40c6-b738-a1f4c74f3aae">
            <rdf:type rdf:resource="http://www.owl-ontologies.com/sumo.owl#Human"/>
            <rdf:type rdf:resource="http://xmlns.com/foaf/0.1/Person"/>
            <pmo:inventorOf rdf:resource="http://example.org/patent/US-H1-H"/>
            <foaf:lastName>Wattana-Chayakul</foaf:lastName>
            <foaf:firstName>Montri</foaf:firstName>
            <schema:address>
               <rdf:Description>
                  <rdf:type rdf:resource="http://schema.org/PostalAddress"/>
                  <schema:addressLocality>Lake Hiawatha</schema:addressLocality>
                  <schema:addressRegion>NJ</schema:addressRegion>
                  <schema:addressCountry rdf:resource="http://example.org/code/country/US"/>
               </rdf:Description>
            </schema:address>
         </rdf:Description>
      </pmo:inventor>
   </rdf:Description>
   <rdf:Description rdf:about="http://example.org/patent/US-H1-H">
      <pmo:assignee>
         <rdf:Description rdf:about="urn:uuid:69973d50-417f-40ac-9476-873ee7db392a">
            <rdf:type rdf:resource="http://www.owl-ontologies.com/sumo.owl#CognitiveAgent"/>
            <rdf:type rdf:resource="http://xmlns.com/foaf/0.1/Organization"/>
            <pmo:assigneeOf rdf:resource="http://example.org/patent/US-H1-H"/>
            <foaf:name>BELL TELEPHONE LABORATORIES, INC.</foaf:name>
            <schema:address>
               <rdf:Description>
                  <rdf:type rdf:resource="http://schema.org/PostalAddress"/>
                  <schema:addressLocality>Murray Hill</schema:addressLocality>
                  <schema:addressRegion>NJ</schema:addressRegion>
                  <schema:addressCountry rdf:resource="http://example.org/code/country/US"/>
               </rdf:Description>
            </schema:address>
         </rdf:Description>
      </pmo:assignee>
   </rdf:Description>
   <rdf:Description rdf:about="http://example.org/patent/US-H1-H">
      <property:agent>
         <rdf:Description rdf:about="urn:uuid:d27ae09f-6db4-4849-8c92-fbcb7585b2a7">
            <rdf:type rdf:resource="http://www.owl-ontologies.com/sumo.owl#Agent"/>
            <rdf:type rdf:resource="http://xmlns.com/foaf/0.1/Agent"/>
            <property:agentOf rdf:resource="http://example.org/patent/US-H1-H"/>
            <foaf:lastName>Roberts</foaf:lastName>
            <foaf:firstName>Patrick E.</foaf:firstName>
         </rdf:Description>
      </property:agent>
   </rdf:Description>
   <rdf:Description rdf:about="http://example.org/patent/US-H1-H">
      <property:hasClaim>
         <rdf:Description rdf:about="http://example.org/patent/US-H1-H/claim/1">
            <rdf:type rdf:resource="http://www.patexpert.org/ontologies/pso.owl#Claim"/>
            <rdf:type rdf:resource="http://www.w3.org/2004/02/skos/core#Concept"/>
            <skos:notation>1</skos:notation>
            <skos:definition xml:lang="en">1. An electrical contact having a cylindrical configuration, having first and second ends and having an open longitudinal wire receiving seam for receipt of two or more wires therein, the improvement comprising;an aperture located in the receiving seam a predetermined distance from said first end of said contact and adapted to release at least one of said wires in the receiving seam as an additional wire is placed in the wire receiving seam.</skos:definition>
         </rdf:Description>
      </property:hasClaim>
   </rdf:Description>
   <rdf:Description rdf:about="http://example.org/patent/US-H1-H">
      <property:hasClaim>
         <rdf:Description rdf:about="http://example.org/patent/US-H1-H/claim/2">
            <rdf:type rdf:resource="http://www.patexpert.org/ontologies/pso.owl#Claim"/>
            <rdf:type rdf:resource="http://www.w3.org/2004/02/skos/core#Concept"/>
            <skos:notation>2</skos:notation>
            <skos:definition xml:lang="en">2. The electrical contact of claim 1 wherein the area of the aperture is larger than a lateral cross-section of wire and its insulation, the wire being used to connect with the electrical contact.</skos:definition>
         </rdf:Description>
      </property:hasClaim>
   </rdf:Description>
   <rdf:Description rdf:about="http://example.org/patent/US-H1-H">
      <property:hasClaim>
         <rdf:Description rdf:about="http://example.org/patent/US-H1-H/claim/3">
            <rdf:type rdf:resource="http://www.patexpert.org/ontologies/pso.owl#Claim"/>
            <rdf:type rdf:resource="http://www.w3.org/2004/02/skos/core#Concept"/>
            <skos:notation>3</skos:notation>
            <skos:definition xml:lang="en">3. The electrical contact of claim 2 further comprising a plurality of locking shoulders located between said first and second ends and nearer to said second end, said locking shoulders comprising sides sloping from said second end towards said first end so as to permit the insertion of said second end through a hole within a base, the locking shoulders adapted to secure said contact within said base after being inserted into said hole.</skos:definition>
         </rdf:Description>
      </property:hasClaim>
   </rdf:Description>
   <rdf:Description rdf:about="http://example.org/patent/US-H1-H">
      <property:hasClaim>
         <rdf:Description rdf:about="http://example.org/patent/US-H1-H/claim/4">
            <rdf:type rdf:resource="http://www.patexpert.org/ontologies/pso.owl#Claim"/>
            <rdf:type rdf:resource="http://www.w3.org/2004/02/skos/core#Concept"/>
            <skos:notation>4</skos:notation>
            <skos:definition xml:lang="en">4. The electrical contact of claim 3 further comprising a tail portion extending below the locking shoulders, the tail portion having a geometry suitable for wire wrap connections.</skos:definition>
         </rdf:Description>
      </property:hasClaim>
   </rdf:Description>
   <rdf:Description rdf:about="http://example.org/patent/US-H1-H">
      <property:hasClaim>
         <rdf:Description rdf:about="http://example.org/patent/US-H1-H/claim/5">
            <rdf:type rdf:resource="http://www.patexpert.org/ontologies/pso.owl#Claim"/>
            <rdf:type rdf:resource="http://www.w3.org/2004/02/skos/core#Concept"/>
            <skos:notation>5</skos:notation>
            <skos:definition xml:lang="en">5. The electrical contact of claim 3 wherein the material of said contact is a phosphor bronze alloy having suitable resilience.</skos:definition>
         </rdf:Description>
      </property:hasClaim>
   </rdf:Description>
   <rdf:Description rdf:about="http://example.org/patent/US-H1-H">
      <property:hasClaim>
         <rdf:Description rdf:about="http://example.org/patent/US-H1-H/claim/6">
            <rdf:type rdf:resource="http://www.patexpert.org/ontologies/pso.owl#Claim"/>
            <rdf:type rdf:resource="http://www.w3.org/2004/02/skos/core#Concept"/>
            <skos:notation>6</skos:notation>
            <skos:definition xml:lang="en">6. A cylindrical electrical terminal of the type which receives wire and is adapted to displace electrical insulation on the wire to make electrical contact thereto, the terminal comprising:an open longitudinal wire receiving seam for receipt of one or more wires therein at its mouth,an aperture located a predetermined distance from the mouth of the receiving seam and defining an area larger than a lateral cross-section of the wire including possible insulation, the aperture positioned to receive and to release the innermost wire from the receiving seam when an additional wire is placed in the receiving seam thereby limiting the wire capacity of the electrical terminal to a predetermined number of wires and releasing connected wires as new wires are engaged in the receiving seam of the electrical terminal.</skos:definition>
         </rdf:Description>
      </property:hasClaim>
   </rdf:Description>
   <rdf:Description rdf:about="http://example.org/patent/US-H1-H">
      <property:hasClaim>
         <rdf:Description rdf:about="http://example.org/patent/US-H1-H/claim/7">
            <rdf:type rdf:resource="http://www.patexpert.org/ontologies/pso.owl#Claim"/>
            <rdf:type rdf:resource="http://www.w3.org/2004/02/skos/core#Concept"/>
            <skos:notation>7</skos:notation>
            <skos:definition xml:lang="en">7. A terminal of the insulation displacing type having a barrel configuration and a longitudinal slot with an entrance for accepting insulated wire to be connected to the terminal, the terminal comprising:an aperture located to communicate with the longitudinal slot a prescribed distance from the entrance of the longitudinal slot and the aperture occupying an area exceeding the cross-sectional area of the wire including the insulation, the predetermined distance being at least long enough to accommodate the dimension occupied by two adjacent wires thereby providing the terminal with the ability to bridge together two wires, the aperture accepting the first of two wires when a third wire is placed in the slot thereby releasing the first wire from the terminal as a third wire is connected to the terminal.</skos:definition>
         </rdf:Description>
      </property:hasClaim>
   </rdf:Description>
   <rdf:Description rdf:about="http://example.org/patent/US-H1-H">
      <property:hasClaim>
         <rdf:Description rdf:about="http://example.org/patent/US-H1-H/claim/8">
            <rdf:type rdf:resource="http://www.patexpert.org/ontologies/pso.owl#Claim"/>
            <rdf:type rdf:resource="http://www.w3.org/2004/02/skos/core#Concept"/>
            <skos:notation>8</skos:notation>
            <skos:definition xml:lang="en">8. A terminal in accordance with claim 7 further comprising:a base of insulative material in a sheet having a first array of apertures, each aperture in the first array adapted to receive a terminal to form an array of terminals.</skos:definition>
         </rdf:Description>
      </property:hasClaim>
   </rdf:Description>
   <rdf:Description rdf:about="http://example.org/patent/US-H1-H">
      <property:hasClaim>
         <rdf:Description rdf:about="http://example.org/patent/US-H1-H/claim/9">
            <rdf:type rdf:resource="http://www.patexpert.org/ontologies/pso.owl#Claim"/>
            <rdf:type rdf:resource="http://www.w3.org/2004/02/skos/core#Concept"/>
            <skos:notation>9</skos:notation>
            <skos:definition xml:lang="en">9. A terminal according to claim 8 further comprising a second sheet of insulation material with a second array of apertures corresponding to the first array, the second sheet having at least one wall-like protrusion aligned with a plurality of the apertures in the second array which extend therethrough, the second sheet adapted to be juxtapositioned with the base and the wall-like protrusion serving as insulating housing for the plurality of terminals inserted therein, each insulating housing having a slot which holds the wire and provides strain relief for preventing breakage of the wire due to flexing in the longitudinal slot.</skos:definition>
         </rdf:Description>
      </property:hasClaim>
   </rdf:Description>
   <rdf:Description rdf:about="http://example.org/patent/US-H1-H">
      <property:hasClaim>
         <rdf:Description rdf:about="http://example.org/patent/US-H1-H/claim/10">
            <rdf:type rdf:resource="http://www.patexpert.org/ontologies/pso.owl#Claim"/>
            <rdf:type rdf:resource="http://www.w3.org/2004/02/skos/core#Concept"/>
            <skos:notation>10</skos:notation>
            <skos:definition xml:lang="en">10. A connector block assembly for split-barrel terminals said connector block having a layered structure comprising:a base member having a plurality of apertures in a first array pattern, each aperture adapted to receive one of the split-barrel terminals,a second member formed from a sheet of insulation material having a plurality of second apertures in a second array pattern adapted to mate with the first array pattern in the base member, the second member having a plurality of wall-like protrusions extending from the second member, each protrusion aligned with one of said second apertures, the second member providing an insulating housing structure for the plurality of terminals with the wall-like protrusions.</skos:definition>
         </rdf:Description>
      </property:hasClaim>
   </rdf:Description>
   <rdf:Description rdf:about="http://example.org/patent/US-H1-H">
      <dcterms:license>User acknowledges that the Information Retrieval Facility (IRF) and its third party providers retain all right, title and interest in and to this xml under applicable copyright laws. User acquires no ownership rights to this xml including but not limited to its format. User hereby accepts the terms and conditions of the Licence Agreement set forth at http://www.ir-facility.org/legal/marec/data_licence</dcterms:license>
   </rdf:Description>
</rdf:RDF>