<?xml version="1.0" encoding="utf-8"?>
<rdf:RDF xmlns:dcterms="http://purl.org/dc/terms/" xmlns:foaf="http://xmlns.com/foaf/0.1/"
         xmlns:prov="http://www.w3.org/ns/prov#"
         xmlns:skos="http://www.w3.org/2004/02/skos/core#"
         xmlns:xkos="http://purl.org/linked-data/xkos#"
         xmlns:pso="http://www.patexpert.org/ontologies/pso.owl#"
         xmlns:rdf="http://www.w3.org/1999/02/22-rdf-syntax-ns#"
         xmlns:pulo="http://www.patexpert.org/ontologies/pulo.owl#"
         xmlns:rdfs="http://www.w3.org/2000/01/rdf-schema#"
         xmlns:sumo="http://www.owl-ontologies.com/sumo.owl#"
         xmlns:owl="http://www.w3.org/2002/07/owl#"
         xmlns:pmo="http://www.patexpert.org/ontologies/pmo.owl#"
         xmlns:xsd="http://www.w3.org/2001/XMLSchema#"
         xmlns:property="http://example.org/property/"
         xmlns:schema="http://schema.org/">
   <rdf:Description rdf:about="http://csarven.ca/#i">
      <rdf:type rdf:resource="http://www.w3.org/ns/prov#Agent"/>
   </rdf:Description>
   <rdf:Description xmlns:xs="http://www.w3.org/2001/XMLSchema"
                    rdf:about="http://example.org/provenance/activity/20130221123112">
      <rdf:type rdf:resource="http://www.w3.org/ns/prov#Activity"/>
      <prov:startedAtTime rdf:datatype="http://www.w3.org/2001/XMLSchema#dateTime">2013-02-21T12:31:12Z</prov:startedAtTime>
      <prov:wasAssociatedWith rdf:resource="http://csarven.ca/#i"/>
      <prov:used rdf:resource="http://example.org/data/EP-1000000-A1.xml"/>
      <prov:used rdf:resource="https://github.com/fusepool/patents-reengineering/src/main/resources/scripts/marec.xsl"/>
      <prov:generated>
         <rdf:Description rdf:about="http://example.org/patent/EP-1000000-A1">
            <prov:wasDerivedFrom rdf:resource="http://example.org/data/EP-1000000-A1.xml"/>
            <prov:wasGeneratedBy rdf:resource="http://example.org/provenance/activity/20130221123112"/>
         </rdf:Description>
      </prov:generated>
   </rdf:Description>
   <rdf:Description rdf:about="http://example.org/patent/EP-1000000-A1">
      <rdf:type rdf:resource="http://www.owl-ontologies.com/sumo.owl#Patent"/>
      <property:status>new</property:status>
      <pmo:patentFamily>
         <rdf:Description rdf:about="http://example.org/family/19768124">
            <rdf:type rdf:resource="http://www.patexpert.org/ontologies/pmo.owl#PatentFamily"/>
            <rdf:type rdf:resource="http://www.w3.org/2004/02/skos/core#Collection"/>
            <skos:notation>19768124</skos:notation>
         </rdf:Description>
      </pmo:patentFamily>
   </rdf:Description>
   <rdf:Description rdf:about="http://example.org/patent/EP-1000000-A1">
      <dcterms:references>
         <rdf:Description rdf:about="http://example.org/patent/EP-1000000-A1/publication">
            <rdf:type rdf:resource="http://www.patexpert.org/ontologies/pmo.owl#IntellectualPropertyDocument"/>
            <property:status>new</property:status>
            <dcterms:hasPart>
               <rdf:Description rdf:about="http://example.org/patent/EP-1000000-A1/publication/20000517">
                  <rdf:type rdf:resource="http://www.patexpert.org/ontologies/pmo.owl#PatentPublication"/>
                  <dcterms:isPartOf rdf:resource="http://example.org/patent/EP-1000000-A1/publication"/>
                  <property:status>new</property:status>
                  <pulo:fileFormat>original</pulo:fileFormat>
                  <property:filing-office rdf:resource="http://example.org/code/filing-office/EP"/>
                  <pmo:publicationNumber>1000000</pmo:publicationNumber>
                  <pmo:kindCode>A1</pmo:kindCode>
                  <rdf:type rdf:resource="http://www.patexpert.org/ontologies/pso.owl#A1Document"/>
                  <pmo:dateOfPublication rdf:datatype="http://www.w3.org/2001/XMLSchema#date">2000-05-17</pmo:dateOfPublication>
               </rdf:Description>
            </dcterms:hasPart>
         </rdf:Description>
      </dcterms:references>
   </rdf:Description>
   <rdf:Description rdf:about="http://example.org/patent/EP-1000000-A1">
      <dcterms:references>
         <rdf:Description rdf:about="http://example.org/patent/EP-99203729-A/application">
            <rdf:type rdf:resource="http://www.patexpert.org/ontologies/pmo.owl#IntellectualPropertyDocument"/>
            <property:status>new</property:status>
            <property:is-representative>NO</property:is-representative>
            <dcterms:hasPart>
               <rdf:Description rdf:about="http://example.org/patent/EP-99203729-A/application/19991108">
                  <rdf:type rdf:resource="http://www.patexpert.org/ontologies/pmo.owl#PatentPublication"/>
                  <dcterms:isPartOf rdf:resource="http://example.org/patent/EP-99203729-A/application"/>
                  <property:status>new</property:status>
                  <pulo:fileFormat>epo</pulo:fileFormat>
                  <property:filing-office rdf:resource="http://example.org/code/filing-office/EP"/>
                  <pmo:applicationNumber>99203729</pmo:applicationNumber>
                  <pmo:dateOfPublication rdf:datatype="http://www.w3.org/2001/XMLSchema#date">1999-11-08</pmo:dateOfPublication>
               </rdf:Description>
            </dcterms:hasPart>
         </rdf:Description>
      </dcterms:references>
   </rdf:Description>
   <rdf:Description rdf:about="http://example.org/patent/EP-1000000-A1">
      <property:priority-claim>
         <rdf:Description rdf:about="http://example.org/patent/NL-1010536-A/publication/1">
            <rdf:type rdf:resource="http://www.patexpert.org/ontologies/pmo.owl#PatentPublication"/>
         </rdf:Description>
      </property:priority-claim>
   </rdf:Description>
   <rdf:Description rdf:about="http://example.org/patent/EP-1000000-A1">
      <pmo:classifiedAs>
         <rdf:Description rdf:about="http://example.org/concept/ecla/B28B1/29">
            <rdf:type rdf:resource="http://www.w3.org/2004/02/skos/core#Concept"/>
            <pmo:classifiedPatent rdf:resource="http://example.org/patent/EP-1000000-A1"/>
            <pmo:classificationCode>B28B1/29</pmo:classificationCode>
            <skos:notation>B28B1/29</skos:notation>
         </rdf:Description>
      </pmo:classifiedAs>
      <pmo:classifiedAs>
         <rdf:Description rdf:about="http://example.org/concept/ecla/B28B5/02B2">
            <rdf:type rdf:resource="http://www.w3.org/2004/02/skos/core#Concept"/>
            <pmo:classifiedPatent rdf:resource="http://example.org/patent/EP-1000000-A1"/>
            <pmo:classificationCode>B28B5/02B2</pmo:classificationCode>
            <skos:notation>B28B5/02B2</skos:notation>
         </rdf:Description>
      </pmo:classifiedAs>
      <pmo:classifiedAs>
         <rdf:Description rdf:about="http://example.org/concept/ecla/B28B7/00F">
            <rdf:type rdf:resource="http://www.w3.org/2004/02/skos/core#Concept"/>
            <pmo:classifiedPatent rdf:resource="http://example.org/patent/EP-1000000-A1"/>
            <pmo:classificationCode>B28B7/00F</pmo:classificationCode>
            <skos:notation>B28B7/00F</skos:notation>
         </rdf:Description>
      </pmo:classifiedAs>
      <pmo:classifiedAs>
         <rdf:Description rdf:about="http://example.org/concept/ecla/H02P6/08">
            <rdf:type rdf:resource="http://www.w3.org/2004/02/skos/core#Concept"/>
            <pmo:classifiedPatent rdf:resource="http://example.org/patent/EP-1000000-A1"/>
            <pmo:classificationCode>H02P6/08</pmo:classificationCode>
            <skos:notation>H02P6/08</skos:notation>
         </rdf:Description>
      </pmo:classifiedAs>
   </rdf:Description>
   <rdf:Description rdf:about="http://example.org/patent/EP-1000000-A1">
      <dcterms:title xml:lang="de">Vorrichtung zur Herstellung von Steinformlingen für die Ziegelindustrie</dcterms:title>
      <dcterms:title xml:lang="en">Apparatus for manufacturing green bricks for the brick manufacturing industry</dcterms:title>
      <dcterms:title xml:lang="fr">Dispositif pour la fabrication de briques crues utilisées dans l'industrie manufacturière des briques</dcterms:title>
   </rdf:Description>
   <rdf:Description rdf:about="http://example.org/patent/EP-1000000-A1">
      <pmo:applicant>
         <rdf:Description rdf:about="urn:uuid:b9f67155-c5fb-4c2c-94ec-bfbef47af13d">
            <rdf:type rdf:resource="http://www.owl-ontologies.com/sumo.owl#CognitiveAgent"/>
            <rdf:type rdf:resource="http://xmlns.com/foaf/0.1/Organization"/>
            <pmo:applicantOf rdf:resource="http://example.org/patent/EP-1000000-A1"/>
            <foaf:name>BOER BEHEER NIJMEGEN BV DE</foaf:name>
            <schema:address>
               <rdf:Description>
                  <rdf:type rdf:resource="http://schema.org/PostalAddress"/>
                  <schema:addressCountry rdf:resource="http://example.org/code/country/NL"/>
               </rdf:Description>
            </schema:address>
         </rdf:Description>
      </pmo:applicant>
   </rdf:Description>
   <rdf:Description rdf:about="http://example.org/patent/EP-1000000-A1">
      <pmo:applicant>
         <rdf:Description rdf:about="urn:uuid:9eb7c178-73dc-4587-a84c-16e50bfaf19a">
            <rdf:type rdf:resource="http://www.owl-ontologies.com/sumo.owl#CognitiveAgent"/>
            <rdf:type rdf:resource="http://xmlns.com/foaf/0.1/Organization"/>
            <pmo:applicantOf rdf:resource="http://example.org/patent/EP-1000000-A1"/>
            <foaf:name>BEHEERMAATSCHAPPIJ DE BOER NIJMEGEN B.V.</foaf:name>
         </rdf:Description>
      </pmo:applicant>
   </rdf:Description>
   <rdf:Description rdf:about="http://example.org/patent/EP-1000000-A1">
      <pmo:applicant>
         <rdf:Description rdf:about="urn:uuid:103ada2e-4475-43ce-a043-b7c7a3992998">
            <rdf:type rdf:resource="http://www.owl-ontologies.com/sumo.owl#CognitiveAgent"/>
            <rdf:type rdf:resource="http://xmlns.com/foaf/0.1/Organization"/>
            <pmo:applicantOf rdf:resource="http://example.org/patent/EP-1000000-A1"/>
            <foaf:lastName>Beheermaatschappij De Boer Nijmegen B.V.</foaf:lastName>
            <schema:address>
               <rdf:Description>
                  <rdf:type rdf:resource="http://schema.org/PostalAddress"/>
                  <schema:streetAddress>Koopvaardijweg 2</schema:streetAddress>
                  <schema:addressLocality>6541 BS Nijmegen</schema:addressLocality>
                  <schema:addressCountry rdf:resource="http://example.org/code/country/NL"/>
               </rdf:Description>
            </schema:address>
         </rdf:Description>
      </pmo:applicant>
   </rdf:Description>
   <rdf:Description rdf:about="http://example.org/patent/EP-1000000-A1">
      <pmo:inventor>
         <rdf:Description rdf:about="urn:uuid:2018781b-a768-49e8-bcdf-bb9d6b1d2667">
            <rdf:type rdf:resource="http://www.owl-ontologies.com/sumo.owl#Human"/>
            <rdf:type rdf:resource="http://xmlns.com/foaf/0.1/Person"/>
            <pmo:inventorOf rdf:resource="http://example.org/patent/EP-1000000-A1"/>
            <foaf:name>KOSMAN WILHELMUS JACOBUS MARIA</foaf:name>
            <schema:address>
               <rdf:Description>
                  <rdf:type rdf:resource="http://schema.org/PostalAddress"/>
                  <schema:addressCountry rdf:resource="http://example.org/code/country/NL"/>
               </rdf:Description>
            </schema:address>
         </rdf:Description>
      </pmo:inventor>
   </rdf:Description>
   <rdf:Description rdf:about="http://example.org/patent/EP-1000000-A1">
      <pmo:inventor>
         <rdf:Description rdf:about="urn:uuid:ba9b92a1-28d4-483e-835a-9d2584ea15d5">
            <rdf:type rdf:resource="http://www.owl-ontologies.com/sumo.owl#Human"/>
            <rdf:type rdf:resource="http://xmlns.com/foaf/0.1/Person"/>
            <pmo:inventorOf rdf:resource="http://example.org/patent/EP-1000000-A1"/>
            <foaf:name>KOSMAN, WILHELMUS JACOBUS MARIA</foaf:name>
         </rdf:Description>
      </pmo:inventor>
   </rdf:Description>
   <rdf:Description rdf:about="http://example.org/patent/EP-1000000-A1">
      <pmo:inventor>
         <rdf:Description rdf:about="urn:uuid:a084b16e-b65a-48f7-b4cf-4e475e8fae84">
            <rdf:type rdf:resource="http://www.owl-ontologies.com/sumo.owl#Human"/>
            <rdf:type rdf:resource="http://xmlns.com/foaf/0.1/Person"/>
            <pmo:inventorOf rdf:resource="http://example.org/patent/EP-1000000-A1"/>
            <foaf:lastName>KOSMAN, WILHELMUS JACOBUS MARIA</foaf:lastName>
            <schema:address>
               <rdf:Description>
                  <rdf:type rdf:resource="http://schema.org/PostalAddress"/>
                  <schema:streetAddress>Bredeweg 9</schema:streetAddress>
                  <schema:addressLocality>6562 DA Groesbeek</schema:addressLocality>
                  <schema:addressCountry rdf:resource="http://example.org/code/country/NL"/>
               </rdf:Description>
            </schema:address>
         </rdf:Description>
      </pmo:inventor>
   </rdf:Description>
   <rdf:Description rdf:about="http://example.org/patent/EP-1000000-A1">
      <property:agent>
         <rdf:Description rdf:about="urn:uuid:f381fbe9-aa67-41d5-bae7-07f25ef8b6c1">
            <rdf:type rdf:resource="http://www.owl-ontologies.com/sumo.owl#Agent"/>
            <rdf:type rdf:resource="http://xmlns.com/foaf/0.1/Agent"/>
            <property:agentOf rdf:resource="http://example.org/patent/EP-1000000-A1"/>
            <foaf:lastName>Schumann, Bernard Herman Johan</foaf:lastName>
            <schema:address>
               <rdf:Description>
                  <rdf:type rdf:resource="http://schema.org/PostalAddress"/>
                  <schema:streetAddress>Arnold &amp;amp; Siedsma, Advocaten en Octrooigemachtigden, Sweelinckplein 1</schema:streetAddress>
                  <schema:addressLocality>2517 GK Den Haag</schema:addressLocality>
                  <schema:addressCountry rdf:resource="http://example.org/code/country/NL"/>
               </rdf:Description>
            </schema:address>
         </rdf:Description>
      </property:agent>
   </rdf:Description>
   <rdf:Description rdf:about="http://example.org/patent/EP-1000000-A1">
      <skos:definition rdf:parseType="Literal">
         <p num="0001">The invention relates to an apparatus for
manufacturing green bricks from clay for the brick
manufacturing industry, comprising a circulating conveyor
carrying mould containers combined to mould container
parts, a reservoir for clay arranged above the mould
containers, means for carrying clay out of the reservoir
into the mould containers, means for pressing and
trimming clay in the mould containers, means for
supplying and placing take-off plates for the green
bricks and means for discharging green bricks released
from the mould containers. Such an apparatus is known in
the field and is for instance described in the patent
1000186 of applicant. The known apparatus is extremely
suitable for automated production of large numbers of
green bricks for the brick manufacturing industry. The
bricks fired from these green bricks have a substantially
smooth, uniform appearance.</p>
         <p num="0002">A recent demand has developed on the market
for bricks which appear as if they have been manufactured
according to traditional methods.</p>
         <p num="0003">The invention has for its object to adapt the
known apparatus such that it can produce in automated
manner large numbers of green bricks with a traditional
appearance.</p>
         <p num="0004">For this purpose the apparatus according to the
invention has the feature that the apparatus further
comprises means for moving the mould container parts
filled with green bricks such that a protruding edge is
formed on at least one side of the green bricks.</p>
         <p num="0005">The bricks fired from the green bricks produced
using the apparatus according to the invention impart
beautiful shadow effects to the wall into which they have 
been built when the sun shines thereon. This aesthetic
effect is an important commercial advantage.</p>
         <p num="0006">The edge-forming means are preferably adapted
to move the mould container parts repeatedly for a
certain period. Repetition a number of times, for
instance three times, is found in practice to be
sufficient to obtain the intended effect.</p>
         <p num="0007">In a practical preferred embodiment the edge-forming
means are adapted to move the mould container
parts substantially transversely of the transporting
direction.</p>
         <p num="0008">In a further preferred embodiment the edge-forming
means comprise a frame which is adapted to engage
individually on a mould container part. This preferred
embodiment has the significant advantage that the edge-forming
means can act on one mould container part while
another mould container part undergoes another operation
and is for instance filled with clay. The edge-forming
means can therefore be added to the known apparatus
without this affecting the production time.</p>
         <p num="0009">In yet another preferred embodiment the frame
spans the mould container part and is provided on both
sides with stop members which are situated during
operation at the location of the side walls of the mould
container part. An exceptionally compact embodiment of
the invention is hereby realized which utilizes the
available space economically and can be arranged without
difficulty on the known apparatus.</p>
         <p num="0010">In order to prevent unnecessary damage to the
mould container parts, these latter are provided on their
side walls with stop surfaces, preferably of plastic. In
preference the stop members of the frame of the edge-forming
means are also provided with these, preferably
plastic, stop surfaces.</p>
         <p num="0011">The invention is described in more detail
hereinbelow with reference to the drawing in which:
<sl>
               <li>figure 1 shows schematically a preferred
embodiment of the apparatus according to the invention; </li>
               <li>figure 2 shows in more detail a perspective
view of a part of the apparatus of figure 1 with the
edge-forming means therein;</li>
               <li>figure 3 shows the edge-forming means of figure
2 in even more detail;</li>
               <li>figure 4 is a perspective view of a first
preferred embodiment of a mould container part which is
suitable for use in the apparatus according to the
invention;</li>
               <li>figure 5 is a perspective view of a second
preferred embodiment of a mould container part; and</li>
               <li>figure 6 shows schematically a part of a wall
which has been built using bricks provided with an edge
and fired from the green bricks manufactured using the
apparatus according to the invention.</li>
            </sl>
         </p>
         <p num="0012">Like components are provided in the figures
with like reference numerals.</p>
         <p num="0013">Figure 1 shows a preferred embodiment of an
apparatus for manufacturing green bricks for the brick
manufacturing industry according to the invention.
Apparatus 1 comprises a conveyor 3. Mould containers
combined to a unit are placed in the form of a mould
container part 4 on the conveyor. The mould container
parts fit closely against each other. Placed above the
mould containers is a reservoir 5 for clay which is kept
in continuous movement by an agitator 6 which is driven
by the electric motor 7. Clay is supplied to reservoir 5
by a circulating conveyor 8. The clay is carried out of
reservoir 5 into the mould containers and then pressed
down by pressing device 9 which is pivotable on shaft 10.
The excess clay is also trimmed using means which are not
drawn. The device 11 carries take-off plates 12 onto a
mould container part such that, after turning over of the
mould container part, the green bricks 13 come to lie on
the plates after being released from the mould
containers.</p>
         <p num="0014">Edge-forming means 22 are arranged between
device 9 and device 11. The edge-forming means move each 
mould container part 4 such that a protruding edge forms
on the upper side of the green bricks received therein.</p>
         <p num="0015">Figure 2 shows in more detail the part of
apparatus 1 comprising edge-forming means 22. In the
shown preferred embodiment, the edge-forming means 22
comprise a frame 26 which spans mould container part 4.
Frame 26 is provided on either side with stop members 27
which are situated at the position of side walls 30 of
the mould container part. The distance between stop
members 27 is greater than the length of the mould
container part. Frame 26 can be moved reciprocally by
means of drive 31 as designated by means of arrow B. In
preference the direction of movement B of frame 26 lies
substantially transversely of the transporting direction
T of conveyor 3. By moving frame 26 repeatedly the stop
members 27 strike alternately against the side walls 30
of the mould container part 4 which is spanned at that
moment by frame 26. As a result the relevant mould
container part is as it were shaken back and forth,
whereby the green bricks 13 situated during operation in
mould containers 21 of mould container part 4 rise a
certain distance in the mould containers. This results in
the intended edge forming on the upper side of each green
brick.</p>
         <p num="0016">Drive 31 is preferably an eccentric drive which
can subject heavy components to a smooth movement owing
to a good distribution of forces. The eccentric drive can
for instance be adjusted such that the moment a stop
member comes up against one of the side walls of a mould
container part, the maximum force is exerted by the drive
on this mould container part.</p>
         <p num="0017">Each mould container part 4 is coupled with
some clearance to conveyor 3 in the direction of movement
B. In the shown preferred embodiment each mould container
part is even disengageably coupled to an associated chain
part 15 of chain conveyor 3. The coupling of both parts
takes place using the bolt-nut connections 16, 17 respectively.
Bolt holes 33 are given an oval form in order to 
create the necessary clearance. Chain part 15 of chain
conveyor 3 comprises ears 18, 19, 20 which serve as links
of the chain conveyor. It is noted that instead of a
chain conveyor many other conveyors known in the field
can be used.</p>
         <p num="0018">Figure 3 shows edge-forming means 22 in even
more detail. So as to prevent damage, stop members 27 are
provided with stop surfaces 28 and corresponding stop
surfaces 29 are arranged on side walls 30 of the mould
container parts. The stop surfaces are preferably of
plastic.</p>
         <p num="0019">Each mould container part 4 is further provided
at both sides with spacer members 32 on walls 30. These
spacer members protrude slightly above the mould container
part itself, so that take-off plates 12 can rest
thereon without damaging the edge which has just been
formed on green bricks 13. It has been found in practice
that the form of green bricks 13, including the edge, is
retained after the mould container part has been turned
over.</p>
         <p num="0020">Figure 4 shows a first preferred embodiment of
a mould container part 4 and a chain part 15 in uncoupled
situation. The different mould containers 21 are combined
to a unit on mould container part 4. It is noted that the
use of edge-forming means 22 has the further important
advantage that additional means for releasing the green
bricks from the mould containers are no longer necessary.
An example of such releasing means known in the field are
bottoms 23 displaceable by means of ejectors 24 such as
are arranged in the second preferred embodiment shown in
figure 5. This ejector lies under bias of spring 25 which
centres the ejector such that no separate guiding is
necessary in chain part 15. Ejector 24 is operated by a
per se known driving device (not shown) during release of
the green bricks. These releasing means are used by
applicant in a number of their apparatuses and are the
subject of the patent 1000186 in the name of applicant.
Figure 5 shows how with some modifications the mould 
container parts and chain parts of the known apparatus
can be used in combination with the edge-forming means
according to the invention. The modifications relate to
enlargement of the holes 34 for ejectors 24 such that
mould container part 4 is coupled to chain part 15 with
some clearance in the direction of movement B. Holes 34
can for instance be oval for this purpose. It is noted
that the multi-part mould container part as described in
applicant's non-prepublished patent application 1007600
can also be made suitable in like manner for use in an
apparatus provided with the edge-forming means according
to the invention.</p>
         <p num="0021">Finally, figure 6 shows a wall 35 which is
built from bricks 36 provided with a protruding edge 37
by using the apparatus according to the invention. It is
possible to imagine that an exceptional shadow effect can
be caused by sunlight incident upon the wall.</p>
         <p num="0022">The present invention is of course not limited
to the described and illustrated embodiment but comprises
all embodiments which fall within the scope of the appended
claims.</p>
      </skos:definition>
      <pso:hasDescriptionSection>
         <rdf:Description rdf:about="http://example.org/patent/EP-1000000-A1/description/0001">
            <rdf:type rdf:resource="http://www.patexpert.org/ontologies/pso.owl#Description"/>
            <skos:notation>0001</skos:notation>
            <skos:definition xml:lang="en">The invention relates to an apparatus for manufacturing green bricks from clay for the brick manufacturing industry, comprising a circulating conveyor carrying mould containers combined to mould container parts, a reservoir for clay arranged above the mould containers, means for carrying clay out of the reservoir into the mould containers, means for pressing and trimming clay in the mould containers, means for supplying and placing take-off plates for the green bricks and means for discharging green bricks released from the mould containers. Such an apparatus is known in the field and is for instance described in the patent 1000186 of applicant. The known apparatus is extremely suitable for automated production of large numbers of green bricks for the brick manufacturing industry. The bricks fired from these green bricks have a substantially smooth, uniform appearance.</skos:definition>
         </rdf:Description>
      </pso:hasDescriptionSection>
      <pso:hasDescriptionSection>
         <rdf:Description rdf:about="http://example.org/patent/EP-1000000-A1/description/0002">
            <rdf:type rdf:resource="http://www.patexpert.org/ontologies/pso.owl#Description"/>
            <skos:notation>0002</skos:notation>
            <skos:definition xml:lang="en">A recent demand has developed on the market for bricks which appear as if they have been manufactured according to traditional methods.</skos:definition>
         </rdf:Description>
      </pso:hasDescriptionSection>
      <pso:hasDescriptionSection>
         <rdf:Description rdf:about="http://example.org/patent/EP-1000000-A1/description/0003">
            <rdf:type rdf:resource="http://www.patexpert.org/ontologies/pso.owl#Description"/>
            <skos:notation>0003</skos:notation>
            <skos:definition xml:lang="en">The invention has for its object to adapt the known apparatus such that it can produce in automated manner large numbers of green bricks with a traditional appearance.</skos:definition>
         </rdf:Description>
      </pso:hasDescriptionSection>
      <pso:hasDescriptionSection>
         <rdf:Description rdf:about="http://example.org/patent/EP-1000000-A1/description/0004">
            <rdf:type rdf:resource="http://www.patexpert.org/ontologies/pso.owl#Description"/>
            <skos:notation>0004</skos:notation>
            <skos:definition xml:lang="en">For this purpose the apparatus according to the invention has the feature that the apparatus further comprises means for moving the mould container parts filled with green bricks such that a protruding edge is formed on at least one side of the green bricks.</skos:definition>
         </rdf:Description>
      </pso:hasDescriptionSection>
      <pso:hasDescriptionSection>
         <rdf:Description rdf:about="http://example.org/patent/EP-1000000-A1/description/0005">
            <rdf:type rdf:resource="http://www.patexpert.org/ontologies/pso.owl#Description"/>
            <skos:notation>0005</skos:notation>
            <skos:definition xml:lang="en">The bricks fired from the green bricks produced using the apparatus according to the invention impart beautiful shadow effects to the wall into which they have been built when the sun shines thereon. This aesthetic effect is an important commercial advantage.</skos:definition>
         </rdf:Description>
      </pso:hasDescriptionSection>
      <pso:hasDescriptionSection>
         <rdf:Description rdf:about="http://example.org/patent/EP-1000000-A1/description/0006">
            <rdf:type rdf:resource="http://www.patexpert.org/ontologies/pso.owl#Description"/>
            <skos:notation>0006</skos:notation>
            <skos:definition xml:lang="en">The edge-forming means are preferably adapted to move the mould container parts repeatedly for a certain period. Repetition a number of times, for instance three times, is found in practice to be sufficient to obtain the intended effect.</skos:definition>
         </rdf:Description>
      </pso:hasDescriptionSection>
      <pso:hasDescriptionSection>
         <rdf:Description rdf:about="http://example.org/patent/EP-1000000-A1/description/0007">
            <rdf:type rdf:resource="http://www.patexpert.org/ontologies/pso.owl#Description"/>
            <skos:notation>0007</skos:notation>
            <skos:definition xml:lang="en">In a practical preferred embodiment the edge-forming means are adapted to move the mould container parts substantially transversely of the transporting direction.</skos:definition>
         </rdf:Description>
      </pso:hasDescriptionSection>
      <pso:hasDescriptionSection>
         <rdf:Description rdf:about="http://example.org/patent/EP-1000000-A1/description/0008">
            <rdf:type rdf:resource="http://www.patexpert.org/ontologies/pso.owl#Description"/>
            <skos:notation>0008</skos:notation>
            <skos:definition xml:lang="en">In a further preferred embodiment the edge-forming means comprise a frame which is adapted to engage individually on a mould container part. This preferred embodiment has the significant advantage that the edge-forming means can act on one mould container part while another mould container part undergoes another operation and is for instance filled with clay. The edge-forming means can therefore be added to the known apparatus without this affecting the production time.</skos:definition>
         </rdf:Description>
      </pso:hasDescriptionSection>
      <pso:hasDescriptionSection>
         <rdf:Description rdf:about="http://example.org/patent/EP-1000000-A1/description/0009">
            <rdf:type rdf:resource="http://www.patexpert.org/ontologies/pso.owl#Description"/>
            <skos:notation>0009</skos:notation>
            <skos:definition xml:lang="en">In yet another preferred embodiment the frame spans the mould container part and is provided on both sides with stop members which are situated during operation at the location of the side walls of the mould container part. An exceptionally compact embodiment of the invention is hereby realized which utilizes the available space economically and can be arranged without difficulty on the known apparatus.</skos:definition>
         </rdf:Description>
      </pso:hasDescriptionSection>
      <pso:hasDescriptionSection>
         <rdf:Description rdf:about="http://example.org/patent/EP-1000000-A1/description/0010">
            <rdf:type rdf:resource="http://www.patexpert.org/ontologies/pso.owl#Description"/>
            <skos:notation>0010</skos:notation>
            <skos:definition xml:lang="en">In order to prevent unnecessary damage to the mould container parts, these latter are provided on their side walls with stop surfaces, preferably of plastic. In preference the stop members of the frame of the edge-forming means are also provided with these, preferably plastic, stop surfaces.</skos:definition>
         </rdf:Description>
      </pso:hasDescriptionSection>
      <pso:hasDescriptionSection>
         <rdf:Description rdf:about="http://example.org/patent/EP-1000000-A1/description/0011">
            <rdf:type rdf:resource="http://www.patexpert.org/ontologies/pso.owl#Description"/>
            <skos:notation>0011</skos:notation>
            <skos:definition xml:lang="en">The invention is described in more detail hereinbelow with reference to the drawing in which: figure 1 shows schematically a preferred embodiment of the apparatus according to the invention; figure 2 shows in more detail a perspective view of a part of the apparatus of figure 1 with the edge-forming means therein;figure 3 shows the edge-forming means of figure 2 in even more detail;figure 4 is a perspective view of a first preferred embodiment of a mould container part which is suitable for use in the apparatus according to the invention;figure 5 is a perspective view of a second preferred embodiment of a mould container part; andfigure 6 shows schematically a part of a wall which has been built using bricks provided with an edge and fired from the green bricks manufactured using the apparatus according to the invention.</skos:definition>
         </rdf:Description>
      </pso:hasDescriptionSection>
      <pso:hasDescriptionSection>
         <rdf:Description rdf:about="http://example.org/patent/EP-1000000-A1/description/0012">
            <rdf:type rdf:resource="http://www.patexpert.org/ontologies/pso.owl#Description"/>
            <skos:notation>0012</skos:notation>
            <skos:definition xml:lang="en">Like components are provided in the figures with like reference numerals.</skos:definition>
         </rdf:Description>
      </pso:hasDescriptionSection>
      <pso:hasDescriptionSection>
         <rdf:Description rdf:about="http://example.org/patent/EP-1000000-A1/description/0013">
            <rdf:type rdf:resource="http://www.patexpert.org/ontologies/pso.owl#Description"/>
            <skos:notation>0013</skos:notation>
            <skos:definition xml:lang="en">Figure 1 shows a preferred embodiment of an apparatus for manufacturing green bricks for the brick manufacturing industry according to the invention. Apparatus 1 comprises a conveyor 3. Mould containers combined to a unit are placed in the form of a mould container part 4 on the conveyor. The mould container parts fit closely against each other. Placed above the mould containers is a reservoir 5 for clay which is kept in continuous movement by an agitator 6 which is driven by the electric motor 7. Clay is supplied to reservoir 5 by a circulating conveyor 8. The clay is carried out of reservoir 5 into the mould containers and then pressed down by pressing device 9 which is pivotable on shaft 10. The excess clay is also trimmed using means which are not drawn. The device 11 carries take-off plates 12 onto a mould container part such that, after turning over of the mould container part, the green bricks 13 come to lie on the plates after being released from the mould containers.</skos:definition>
         </rdf:Description>
      </pso:hasDescriptionSection>
      <pso:hasDescriptionSection>
         <rdf:Description rdf:about="http://example.org/patent/EP-1000000-A1/description/0014">
            <rdf:type rdf:resource="http://www.patexpert.org/ontologies/pso.owl#Description"/>
            <skos:notation>0014</skos:notation>
            <skos:definition xml:lang="en">Edge-forming means 22 are arranged between device 9 and device 11. The edge-forming means move each mould container part 4 such that a protruding edge forms on the upper side of the green bricks received therein.</skos:definition>
         </rdf:Description>
      </pso:hasDescriptionSection>
      <pso:hasDescriptionSection>
         <rdf:Description rdf:about="http://example.org/patent/EP-1000000-A1/description/0015">
            <rdf:type rdf:resource="http://www.patexpert.org/ontologies/pso.owl#Description"/>
            <skos:notation>0015</skos:notation>
            <skos:definition xml:lang="en">Figure 2 shows in more detail the part of apparatus 1 comprising edge-forming means 22. In the shown preferred embodiment, the edge-forming means 22 comprise a frame 26 which spans mould container part 4. Frame 26 is provided on either side with stop members 27 which are situated at the position of side walls 30 of the mould container part. The distance between stop members 27 is greater than the length of the mould container part. Frame 26 can be moved reciprocally by means of drive 31 as designated by means of arrow B. In preference the direction of movement B of frame 26 lies substantially transversely of the transporting direction T of conveyor 3. By moving frame 26 repeatedly the stop members 27 strike alternately against the side walls 30 of the mould container part 4 which is spanned at that moment by frame 26. As a result the relevant mould container part is as it were shaken back and forth, whereby the green bricks 13 situated during operation in mould containers 21 of mould container part 4 rise a certain distance in the mould containers. This results in the intended edge forming on the upper side of each green brick.</skos:definition>
         </rdf:Description>
      </pso:hasDescriptionSection>
      <pso:hasDescriptionSection>
         <rdf:Description rdf:about="http://example.org/patent/EP-1000000-A1/description/0016">
            <rdf:type rdf:resource="http://www.patexpert.org/ontologies/pso.owl#Description"/>
            <skos:notation>0016</skos:notation>
            <skos:definition xml:lang="en">Drive 31 is preferably an eccentric drive which can subject heavy components to a smooth movement owing to a good distribution of forces. The eccentric drive can for instance be adjusted such that the moment a stop member comes up against one of the side walls of a mould container part, the maximum force is exerted by the drive on this mould container part.</skos:definition>
         </rdf:Description>
      </pso:hasDescriptionSection>
      <pso:hasDescriptionSection>
         <rdf:Description rdf:about="http://example.org/patent/EP-1000000-A1/description/0017">
            <rdf:type rdf:resource="http://www.patexpert.org/ontologies/pso.owl#Description"/>
            <skos:notation>0017</skos:notation>
            <skos:definition xml:lang="en">Each mould container part 4 is coupled with some clearance to conveyor 3 in the direction of movement B. In the shown preferred embodiment each mould container part is even disengageably coupled to an associated chain part 15 of chain conveyor 3. The coupling of both parts takes place using the bolt-nut connections 16, 17 respectively. Bolt holes 33 are given an oval form in order to create the necessary clearance. Chain part 15 of chain conveyor 3 comprises ears 18, 19, 20 which serve as links of the chain conveyor. It is noted that instead of a chain conveyor many other conveyors known in the field can be used.</skos:definition>
         </rdf:Description>
      </pso:hasDescriptionSection>
      <pso:hasDescriptionSection>
         <rdf:Description rdf:about="http://example.org/patent/EP-1000000-A1/description/0018">
            <rdf:type rdf:resource="http://www.patexpert.org/ontologies/pso.owl#Description"/>
            <skos:notation>0018</skos:notation>
            <skos:definition xml:lang="en">Figure 3 shows edge-forming means 22 in even more detail. So as to prevent damage, stop members 27 are provided with stop surfaces 28 and corresponding stop surfaces 29 are arranged on side walls 30 of the mould container parts. The stop surfaces are preferably of plastic.</skos:definition>
         </rdf:Description>
      </pso:hasDescriptionSection>
      <pso:hasDescriptionSection>
         <rdf:Description rdf:about="http://example.org/patent/EP-1000000-A1/description/0019">
            <rdf:type rdf:resource="http://www.patexpert.org/ontologies/pso.owl#Description"/>
            <skos:notation>0019</skos:notation>
            <skos:definition xml:lang="en">Each mould container part 4 is further provided at both sides with spacer members 32 on walls 30. These spacer members protrude slightly above the mould container part itself, so that take-off plates 12 can rest thereon without damaging the edge which has just been formed on green bricks 13. It has been found in practice that the form of green bricks 13, including the edge, is retained after the mould container part has been turned over.</skos:definition>
         </rdf:Description>
      </pso:hasDescriptionSection>
      <pso:hasDescriptionSection>
         <rdf:Description rdf:about="http://example.org/patent/EP-1000000-A1/description/0020">
            <rdf:type rdf:resource="http://www.patexpert.org/ontologies/pso.owl#Description"/>
            <skos:notation>0020</skos:notation>
            <skos:definition xml:lang="en">Figure 4 shows a first preferred embodiment of a mould container part 4 and a chain part 15 in uncoupled situation. The different mould containers 21 are combined to a unit on mould container part 4. It is noted that the use of edge-forming means 22 has the further important advantage that additional means for releasing the green bricks from the mould containers are no longer necessary. An example of such releasing means known in the field are bottoms 23 displaceable by means of ejectors 24 such as are arranged in the second preferred embodiment shown in figure 5. This ejector lies under bias of spring 25 which centres the ejector such that no separate guiding is necessary in chain part 15. Ejector 24 is operated by a per se known driving device (not shown) during release of the green bricks. These releasing means are used by applicant in a number of their apparatuses and are the subject of the patent 1000186 in the name of applicant. Figure 5 shows how with some modifications the mould container parts and chain parts of the known apparatus can be used in combination with the edge-forming means according to the invention. The modifications relate to enlargement of the holes 34 for ejectors 24 such that mould container part 4 is coupled to chain part 15 with some clearance in the direction of movement B. Holes 34 can for instance be oval for this purpose. It is noted that the multi-part mould container part as described in applicant's non-prepublished patent application 1007600 can also be made suitable in like manner for use in an apparatus provided with the edge-forming means according to the invention.</skos:definition>
         </rdf:Description>
      </pso:hasDescriptionSection>
      <pso:hasDescriptionSection>
         <rdf:Description rdf:about="http://example.org/patent/EP-1000000-A1/description/0021">
            <rdf:type rdf:resource="http://www.patexpert.org/ontologies/pso.owl#Description"/>
            <skos:notation>0021</skos:notation>
            <skos:definition xml:lang="en">Finally, figure 6 shows a wall 35 which is built from bricks 36 provided with a protruding edge 37 by using the apparatus according to the invention. It is possible to imagine that an exceptional shadow effect can be caused by sunlight incident upon the wall.</skos:definition>
         </rdf:Description>
      </pso:hasDescriptionSection>
      <pso:hasDescriptionSection>
         <rdf:Description rdf:about="http://example.org/patent/EP-1000000-A1/description/0022">
            <rdf:type rdf:resource="http://www.patexpert.org/ontologies/pso.owl#Description"/>
            <skos:notation>0022</skos:notation>
            <skos:definition xml:lang="en">The present invention is of course not limited to the described and illustrated embodiment but comprises all embodiments which fall within the scope of the appended claims.</skos:definition>
         </rdf:Description>
      </pso:hasDescriptionSection>
   </rdf:Description>
   <rdf:Description rdf:about="http://example.org/patent/EP-1000000-A1">
      <property:hasClaim>
         <rdf:Description rdf:about="http://example.org/patent/EP-1000000-A1/claim/1">
            <rdf:type rdf:resource="http://www.patexpert.org/ontologies/pso.owl#Claim"/>
            <rdf:type rdf:resource="http://www.w3.org/2004/02/skos/core#Concept"/>
            <skos:notation>1</skos:notation>
            <skos:definition xml:lang="en">Apparatus for manufacturing green bricks from clay for the brick manufacturing industry, comprising a circulating conveyor carrying mould containers combined to mould container parts, a reservoir for clay arranged above the mould containers, means for carrying clay out of the reservoir into the mould containers, means for pressing and trimming clay in the mould containers, means for supplying and placing take-off plates for the green bricks and means for discharging green bricks released from the mould containers, characterized in that the apparatus further comprises means for moving the mould container parts filled with green bricks such that a protruding edge is formed on at least one side of the green bricks.</skos:definition>
         </rdf:Description>
      </property:hasClaim>
   </rdf:Description>
   <rdf:Description rdf:about="http://example.org/patent/EP-1000000-A1">
      <property:hasClaim>
         <rdf:Description rdf:about="http://example.org/patent/EP-1000000-A1/claim/2">
            <rdf:type rdf:resource="http://www.patexpert.org/ontologies/pso.owl#Claim"/>
            <rdf:type rdf:resource="http://www.w3.org/2004/02/skos/core#Concept"/>
            <skos:notation>2</skos:notation>
            <skos:definition xml:lang="en">Apparatus as claimed in claim 1, wherein the edge-forming means are adapted to move the mould container parts repeatedly for a certain period.</skos:definition>
         </rdf:Description>
      </property:hasClaim>
   </rdf:Description>
   <rdf:Description rdf:about="http://example.org/patent/EP-1000000-A1">
      <property:hasClaim>
         <rdf:Description rdf:about="http://example.org/patent/EP-1000000-A1/claim/3">
            <rdf:type rdf:resource="http://www.patexpert.org/ontologies/pso.owl#Claim"/>
            <rdf:type rdf:resource="http://www.w3.org/2004/02/skos/core#Concept"/>
            <skos:notation>3</skos:notation>
            <skos:definition xml:lang="en">Apparatus as claimed in claim 1 or 2, wherein the edge-forming means are adapted to move the mould container parts substantially transversely of the transporting direction.</skos:definition>
         </rdf:Description>
      </property:hasClaim>
   </rdf:Description>
   <rdf:Description rdf:about="http://example.org/patent/EP-1000000-A1">
      <property:hasClaim>
         <rdf:Description rdf:about="http://example.org/patent/EP-1000000-A1/claim/4">
            <rdf:type rdf:resource="http://www.patexpert.org/ontologies/pso.owl#Claim"/>
            <rdf:type rdf:resource="http://www.w3.org/2004/02/skos/core#Concept"/>
            <skos:notation>4</skos:notation>
            <skos:definition xml:lang="en">Apparatus as claimed in any of the foregoing claims, wherein the edge-forming means comprise a frame which is adapted to engage individually on a mould container part.</skos:definition>
         </rdf:Description>
      </property:hasClaim>
   </rdf:Description>
   <rdf:Description rdf:about="http://example.org/patent/EP-1000000-A1">
      <property:hasClaim>
         <rdf:Description rdf:about="http://example.org/patent/EP-1000000-A1/claim/5">
            <rdf:type rdf:resource="http://www.patexpert.org/ontologies/pso.owl#Claim"/>
            <rdf:type rdf:resource="http://www.w3.org/2004/02/skos/core#Concept"/>
            <skos:notation>5</skos:notation>
            <skos:definition xml:lang="en">Apparatus as claimed in claim 4, wherein the frame spans the mould container part and is provided on both sides with stop members which are situated during operation at the location of the side walls of the mould container part.</skos:definition>
         </rdf:Description>
      </property:hasClaim>
   </rdf:Description>
   <rdf:Description rdf:about="http://example.org/patent/EP-1000000-A1">
      <property:hasClaim>
         <rdf:Description rdf:about="http://example.org/patent/EP-1000000-A1/claim/6">
            <rdf:type rdf:resource="http://www.patexpert.org/ontologies/pso.owl#Claim"/>
            <rdf:type rdf:resource="http://www.w3.org/2004/02/skos/core#Concept"/>
            <skos:notation>6</skos:notation>
            <skos:definition xml:lang="en">Apparatus as claimed in claim 5, wherein the stop members are provided with stop surfaces which preferably comprise plastic.</skos:definition>
         </rdf:Description>
      </property:hasClaim>
   </rdf:Description>
   <rdf:Description rdf:about="http://example.org/patent/EP-1000000-A1">
      <property:hasClaim>
         <rdf:Description rdf:about="http://example.org/patent/EP-1000000-A1/claim/7">
            <rdf:type rdf:resource="http://www.patexpert.org/ontologies/pso.owl#Claim"/>
            <rdf:type rdf:resource="http://www.w3.org/2004/02/skos/core#Concept"/>
            <skos:notation>7</skos:notation>
            <skos:definition xml:lang="en">Apparatus as claimed in claim 5 or 6, wherein the mould container parts are provided on their side walls with stop surfaces which preferably comprise plastic.</skos:definition>
         </rdf:Description>
      </property:hasClaim>
   </rdf:Description>
   <rdf:Description rdf:about="http://example.org/patent/EP-1000000-A1">
      <property:hasClaim>
         <rdf:Description rdf:about="http://example.org/patent/EP-1000000-A1/claim/8">
            <rdf:type rdf:resource="http://www.patexpert.org/ontologies/pso.owl#Claim"/>
            <rdf:type rdf:resource="http://www.w3.org/2004/02/skos/core#Concept"/>
            <skos:notation>8</skos:notation>
            <skos:definition xml:lang="en">Apparatus as claimed in claim 4, 5, 6 or 7, wherein the edge-forming means comprise an eccentric drive for the frame.</skos:definition>
         </rdf:Description>
      </property:hasClaim>
   </rdf:Description>
   <rdf:Description rdf:about="http://example.org/patent/EP-1000000-A1">
      <property:hasClaim>
         <rdf:Description rdf:about="http://example.org/patent/EP-1000000-A1/claim/9">
            <rdf:type rdf:resource="http://www.patexpert.org/ontologies/pso.owl#Claim"/>
            <rdf:type rdf:resource="http://www.w3.org/2004/02/skos/core#Concept"/>
            <skos:notation>9</skos:notation>
            <skos:definition xml:lang="en">Apparatus as claimed in any of the foregoing claims, wherein each mould container part is provided with a number of spacer members for supporting the take-off plates at a distance above the green bricks.</skos:definition>
         </rdf:Description>
      </property:hasClaim>
   </rdf:Description>
   <rdf:Description rdf:about="http://example.org/patent/EP-1000000-A1">
      <property:hasClaim>
         <rdf:Description rdf:about="http://example.org/patent/EP-1000000-A1/claim/10">
            <rdf:type rdf:resource="http://www.patexpert.org/ontologies/pso.owl#Claim"/>
            <rdf:type rdf:resource="http://www.w3.org/2004/02/skos/core#Concept"/>
            <skos:notation>10</skos:notation>
            <skos:definition xml:lang="en">Apparatus as claimed in any of the foregoing claims, wherein the mould container parts are fixed movably onto the conveyor with some clearance in the direction of movement.</skos:definition>
         </rdf:Description>
      </property:hasClaim>
   </rdf:Description>
   <rdf:Description rdf:about="http://example.org/patent/EP-1000000-A1">
      <property:hasClaim>
         <rdf:Description rdf:about="http://example.org/patent/EP-1000000-A1/claim/11">
            <rdf:type rdf:resource="http://www.patexpert.org/ontologies/pso.owl#Claim"/>
            <rdf:type rdf:resource="http://www.w3.org/2004/02/skos/core#Concept"/>
            <skos:notation>11</skos:notation>
            <skos:definition xml:lang="en">Apparatus as claimed in claim 10, wherein the conveyor is a chain conveyor and the mould container parts are coupled with some clearance in the direction of movement to a chain part connectable to the chain.</skos:definition>
         </rdf:Description>
      </property:hasClaim>
   </rdf:Description>
   <rdf:Description rdf:about="http://example.org/patent/EP-1000000-A1">
      <dcterms:license>User acknowledges that the Information Retrieval Facility (IRF) and its third party providers retain all right, title and interest in and to this xml under applicable copyright laws. User acquires no ownership rights to this xml including but not limited to its format. User hereby accepts the terms and conditions of the Licence Agreement set forth at http://www.ir-facility.org/legal/marec/data_licence</dcterms:license>
   </rdf:Description>
</rdf:RDF>